



lee215

★ 47713

Last Edit: November 16, 2019 10:00 PM 1.4K VIEWS

50

## Solution 1: Recursion idea

The following sequence can be built up from the earlier result.

So I search index of the prefix part

For example:

$f(5) = "10"$

$f(6) = "11"$

The prefix are both  $f(2) = "1"$

so we found that  $f(n)$  has  $f((n - 1) / 2)$  as prefix.

## Java:

```
public String encode(int n) {
    return n > 0 ? encode((n - 1) / 2) + "10".charAt(n % 2) : "";
}
```

## C++:

```
string encode(int n) {
    return n > 0 ? encode((n - 1) / 2) + "10"[n % 2] : "";
}
```

## Python:

```
def encode(self, n):
    return self.encode((n - 1) / 2) + '10'[n % 2] if n else ""
```

Solution 2: Binary of  $n + 1$ 

Assume  $g(n) = "1" + f(n)$

we can find:

$g(0) = "1"$   $g(1) = "10"$   $g(2) = "111"$   $g(3) = "100"$   $g(4) = "101"$   $g(5) = "110"$   $g(6) = "111"$

Now everything is obvious:

$g(n) = \text{binary}(n + 1)$

$"1" + f(n) = \text{binary}(n + 1)$

$f(n) = \text{binary}(n + 1).substring(1)$

## Java:

```
public String encode(int n) {
    return Integer.toBinaryString(n + 1).substring(1);
}
```

## Python:

```
def encode(self, n):
    return bin(n + 1)[3:]
```

## Complexity

Time  $O(\log N)$

Space  $O(\log N)$

## More

Thanks for upvotes and followers.

weibo leetcode